crypto_examples/mulntt_ct/mulntt_ct.dfy
@@ -1,4 +1,3 @@
-include "nth_root.dfy"
 include "mulntt_ct_rec.dfy"
 
 module ntt {
@@ -9,13 +8,14 @@ module ntt {
     import opened Mul
 
     import opened pows_of_2
-    import opened omegas
+    import opened nth_root
+    import opened ntt_index
 
     import opened mulntt_ct_rec
     // import opened ntt_recs
     // import opened rindex
     // import opened bins
-    // import opened polys
+    import opened polys
 
     function method block_count(m: pow2_t): nat
         requires 0 <= m.exp <= LOGN;
@@ -55,24 +55,94 @@ module ntt {
 
     type n_sized = s: seq<elem>
         | |s| == N == pow2(LOGN).full witness *
+    
+    lemma point_view_index_bound_lemma(i: nat, j: nat, bsize: pow2_t)
+        requires bsize.exp <= LOGN;
+        requires i < block_count(bsize);
+        requires j < bsize.full;
+        ensures 0 <= i + j * block_count(bsize) < N;
+    {
+        var count := block_count(bsize);
+        calc {
+            i + j * count;
+            <=
+            count - 1 + j * count;
+            <= { LemmaMulInequality(j, bsize.full - 1, count); }
+            count - 1 + (bsize.full - 1) * count;
+            { LemmaMulIsDistributive(count, bsize.full, 1); }
+            count - 1 + bsize.full * count - count;
+            bsize.full * count - 1;
+            { Nth_root_lemma(); }
+            N - 1;
+        }
+
+        LemmaMulStrictlyPositiveAuto();
+    }
+
+    function point_view_index(i: nat, j: nat, bsize: pow2_t): (offset: nat)
+        requires bsize.exp <= LOGN;
+        requires i < block_count(bsize);
+        requires j < bsize.full;
+        ensures offset < N;
+    {
+        point_view_index_bound_lemma(i, j, bsize);
+        i + j * block_count(bsize)
+    }
+
+    function points_view(a: n_sized, i: nat, bsize: pow2_t): (v: seq<elem>)
+        requires bsize.exp <= LOGN;
+        requires i < block_count(bsize);
+        // ensures |v| == bsize.full;
+    {
+        var size := bsize.full;
+        seq(size, j requires 0 <= j < size => a[point_view_index(i, j, bsize)])
+    }
+
+    function level_points_view(a: n_sized, bsize: pow2_t): (vs: seq<seq<elem>>)
+        requires bsize.exp <= LOGN;
+        ensures unifromly_sized(vs, bsize);
+    {
+        var count := block_count(bsize);
+        var vs := seq(count, i requires 0 <= i < count => points_view(a, i, bsize));
+        assert unifromly_sized(vs, bsize) by {
+            reveal unifromly_sized();
+        }
+        vs
+    }
+
+    function x_value(i: nat, bsize: pow2_t): elem
+        requires bsize.exp <= LOGN;
+        requires i < bsize.full;
+    {
+        var count := block_count(bsize);
+        LemmaMulNonnegative(count, bit_rev_int(i, bsize));
+        modmul(modpow(OMEGA, count * bit_rev_int(i, bsize)), modpow(PSI, count))
+    }
+
+    predicate points_eval_inv(points: seq<elem>, poly: seq<elem>, bsize: pow2_t, k: nat)
+        requires bsize.exp <= LOGN;
+        requires k <= |points| == |poly| == bsize.full;
+    {
+        forall i | 0 <= i < k :: poly_eval(poly, x_value(i, bsize)) == points[i]
+    }
 
     function method A(): n_sized
 
     function method P(): n_sized
 
-    lemma A_table_index_bounded_lemma(s: nat, d: pow2_t, j: nat, t: pow2_t)
-        requires 0 <= d.exp < LOGN;
-        requires 0 <= t.exp < LOGN;
-        requires block_count(t) == 2 * d.full;
-        // requires block_count(pow2_double(t)) == d.full;
-        requires j < t.full;
-        requires s < (2 * d.full) * j + d.full;
-        ensures s + d.full < N;
-    {
-        assume false;
-        // block_count_product_lemma(t);
-        // assert block_count(t) * t.full == N;
-    }
+    // lemma A_table_index_bounded_lemma(s: nat, d: pow2_t, j: nat, t: pow2_t)
+    //     requires 0 <= d.exp < LOGN;
+    //     requires 0 <= t.exp < LOGN;
+    //     requires block_count(t) == 2 * d.full;
+    //     // requires block_count(pow2_double(t)) == d.full;
+    //     requires j < t.full;
+    //     requires s < (2 * d.full) * j + d.full;
+    //     ensures s + d.full < N;
+    // {
+    //     assume false;
+    //     // block_count_product_lemma(t);
+    //     // assert block_count(t) * t.full == N;
+    // }
 
     datatype slice_loop_view = slice_loop_view(
         lower: lpolys,
@@ -85,72 +155,94 @@ module ntt {
             && 1 <= higher.bsize.exp <= LOGN
             && higher.build_smaller_level() == lower
         }
-    }
 
-    // predicate slice_loop_inv()
-
-    function bit_rev_int(j: nat, bound: pow2_t): nat
-
-    method slice_loop(
-        a: n_sized,
-        u: nat,
-        d: pow2_t,
-        w: elem,
-        ghost j: nat,
-        ghost t: pow2_t)
-        // ghost sv: slice_loop_view)
-
-    returns (new_a: n_sized)
-    
-    // ghost new_blocks: seq<seq<elem>>)
-        // requires |blocks| == d.full;
-        requires 0 <= t.exp < LOGN;
-        requires 0 <= d.exp < LOGN;
-
-        requires 2 * d.full * bit_rev_int(j, t) >= 0;
-
-        requires block_count(t) == 2 * d.full;
-        // d blocks, each of 2t size 
-        // requires block_count(pow2_double(t)) == d.full;
-        requires j < t.full;
-        requires u == (2 * d.full) * j;
-        // requires t.exp == 0 ==> a == A();
-
-        // ensures |new_blocks| == d.full;
-    {
-        var s := u;
-        // new_blocks := blocks;
-        new_a := a;
-
-        assume w == modpow(PSI, 2 * d.full * bit_rev_int(j, t) + d.full);
-
-        while (s < u + d.full)
-            // invariant |new_blocks| == |blocks|;
-            // invariant 
+        function get_even_poly(which: nat): (r: seq<elem>)
+            requires slice_view_wf();
+            requires which < |higher.blocks|;
+            ensures |higher.blocks[which]| == higher.bsize.full;
+            ensures r == even_indexed_items(higher.blocks[which], higher.bsize);
         {
-            A_table_index_bounded_lemma(s, d, j, t);
-            ghost var b_idx := s - u;
-            var e := a[s];
-            var o := a[s + d.full];
+            higher.level_index_correspondence_lemma(which, lower);
+            lower.blocks[2 * which]
+        }
 
-            // assume e == 
-
-            var x := modmul(o, w);
-            new_a := new_a[s+d.full := modsub(e, x)];
-            new_a := new_a[s := modadd(e, x)];
-
-            s := s + 1;
-            // new_blocks := new_blocks[b_idx := blocks[b_idx]];
+        function get_odd_poly(which: nat): (r: seq<elem>)
+            requires slice_view_wf();
+            requires which < |higher.blocks|;
+            ensures |higher.blocks[which]| == higher.bsize.full;
+            ensures r == odd_indexed_items(higher.blocks[which], higher.bsize);
+        {
+            higher.level_index_correspondence_lemma(which, lower);
+            lower.blocks[2 * which + 1]
         }
     }
 
-    lemma P_table_index_bounded_lemma(t: pow2_t, j: nat)
-        requires t.exp < LOGN;
-        requires j < t.full;
-        ensures t.full + j < N;
-    {
-        assume false;
-    }
+    function bit_rev_int(j: nat, bound: pow2_t): nat
+
+    // method slice_loop(
+    //     a: n_sized,
+    //     u: nat,
+    //     d: pow2_t,
+    //     w: elem,
+    //     ghost j: nat,
+    //     ghost t: pow2_t,
+    //     ghost sv: slice_loop_view)
+
+    // returns (new_a: n_sized)
+    
+    // // ghost new_blocks: seq<seq<elem>>)
+    //     // requires |blocks| == d.full;
+    //     requires 0 <= t.exp < LOGN;
+    //     requires 0 <= d.exp < LOGN;
+
+    //     requires 2 * d.full * bit_rev_int(j, t) >= 0;
+
+    //     requires block_count(t) == 2 * d.full;
+    //     // d blocks, each of 2t size 
+    //     // requires block_count(pow2_double(t)) == d.full;
+    //     requires j < t.full;
+    //     requires u == (2 * d.full) * j;
+
+    //     requires sv.slice_view_wf();
+    //     // requires t.exp == 0 ==> a == A(); // not quite right
+
+    //     // ensures |new_blocks| == d.full;
+    // {
+    //     var s := u;
+    //     // new_blocks := blocks;
+    //     new_a := a;
+
+    //     assume w == modpow(PSI, 2 * d.full * bit_rev_int(j, t) + d.full);
+
+    //     while (s < u + d.full)
+    //         // invariant |new_blocks| == |blocks|;
+    //         // invariant 
+    //     {
+    //         A_table_index_bounded_lemma(s, d, j, t);
+    //         ghost var b_idx := s - u;
+    //         var e := a[s];
+    //         var o := a[s + d.full];
+
+    //         var xe = (pow(OMEGA, d * bit_rev_int(2*j, logn), Q) * pow(PSI, d, Q)) % Q;
+
+    //         // assume e == ;
+
+    //         var x := modmul(o, w);
+    //         new_a := new_a[s+d.full := modsub(e, x)];
+    //         new_a := new_a[s := modadd(e, x)];
+
+    //         s := s + 1;
+    //         // new_blocks := new_blocks[b_idx := blocks[b_idx]];
+    //     }
+    // }
+
+    // lemma P_table_index_bounded_lemma(t: pow2_t, j: nat)
+    //     requires t.exp < LOGN;
+    //     requires j < t.full;
+    //     ensures t.full + j < N;
+    // {
+    //     assume false;
+    // }
 
     // method level_loop(a: n_sized, t: pow2_t, d: pow2_t)
     //     requires t.exp < LOGN;
