crypto_examples/mulntt_ct/mulntt_ct_rec.dfy
@@ -1,4 +1,6 @@
 include "nth_root.dfy"
+include "ntt_index.dfy"
+include "polys.dfy"
 
 module mulntt_ct_rec {
     import opened Seq
@@ -8,24 +10,11 @@ module mulntt_ct_rec {
     import opened Mul
 
     import opened pows_of_2
-    import opened omegas
 
+    import opened nth_root
+    import opened ntt_index
     // function method A(): seq<elem>
     //     ensures |A()| == N == pow2(LOGN).full;
-
-    function method {:opaque} even_indexed_items<T>(a: seq<T>, len: pow2_t): seq<T>
-        requires |a| == len.full;
-    {
-        pow2_basics(len);
-        seq(len.full/2, n requires 0 <= n < len.full/2 => a[n * 2])
-    }
-
-    function method {:opaque} odd_indexed_items<T>(a: seq<T>, len: pow2_t): seq<T>
-        requires |a| == len.full;
-    {
-        pow2_basics(len);
-        seq(len.full/2, n requires 0 <= n < len.full/2 => a[n * 2 + 1])
-    }
 
     function method block_count(m: pow2_t): nat
         requires 0 <= m.exp <= LOGN;
@@ -58,9 +47,9 @@ module mulntt_ct_rec {
 
     datatype lpolys = lpolys_cons(blocks: seq<seq<elem>>, bsize: pow2_t)
     {
-        predicate {:opaque} level_wf()
+        predicate level_wf()
         {
-            && (forall i: nat | i < |blocks| :: |blocks[i]| == bsize.full)
+            && unifromly_sized(blocks, bsize)
             && 0 <= bsize.exp <= LOGN
             && block_count(bsize) == |blocks|
         }
@@ -70,8 +59,9 @@ module mulntt_ct_rec {
             requires 1 <= bsize.exp <= LOGN;
             ensures lps.level_wf();
             ensures lps.bsize == pow2_half(bsize);
+            ensures |lps.blocks| == 2 * |blocks|;
         {
-            reveal level_wf();
+            reveal unifromly_sized();
             pow2_basics(bsize);
             block_count_half_lemma(bsize);
             var new_size := pow2_half(bsize);
@@ -79,11 +69,7 @@ module mulntt_ct_rec {
             var new_blocks := seq(new_count, n requires 0 <= n < new_count => 
                 if n % 2 == 0 then even_indexed_items(blocks[n/2], bsize)
                 else odd_indexed_items(blocks[n/2], bsize));
-            var l := lpolys_cons(new_blocks, new_size);
-            assert l.level_wf() by {
-                reveal l.level_wf();
-            }
-            l
+            lpolys_cons(new_blocks, new_size)
         }
 
         // lemma base_level_correct()
@@ -104,11 +90,12 @@ module mulntt_ct_rec {
             ensures |blocks[i]| == bsize.full;
             ensures 2 * i + 1 < |sl.blocks|;
             ensures even_indexed_items(blocks[i], bsize) == sl.blocks[2 * i];
+            ensures |sl.blocks[2 * i]| == pow2_half(bsize).full;
             ensures odd_indexed_items(blocks[i], bsize) == sl.blocks[2 * i + 1];
+            ensures |sl.blocks[2 * i + 1]| == pow2_half(bsize).full;
         {
-            reveal level_wf();
+            reveal unifromly_sized();
             reveal build_smaller_level();
-            reveal sl.level_wf();
         }
     }
 
