crypto_examples/mulntt_ct/ntt_index.dfy
@@ -1,0 +1,28 @@
+include "nth_root.dfy"
+include "../ntt_cleanup/pow2.dfy"
+
+module ntt_index {
+    import opened Seq
+
+    import opened nth_root
+    import opened pows_of_2
+
+    function method {:opaque} even_indexed_items<T>(a: seq<T>, len: pow2_t): seq<T>
+        requires |a| == len.full;
+    {
+        pow2_basics(len);
+        seq(len.full/2, n requires 0 <= n < len.full/2 => a[n * 2])
+    }
+
+    function method {:opaque} odd_indexed_items<T>(a: seq<T>, len: pow2_t): seq<T>
+        requires |a| == len.full;
+    {
+        pow2_basics(len);
+        seq(len.full/2, n requires 0 <= n < len.full/2 => a[n * 2 + 1])
+    }
+
+    predicate {:opaque} unifromly_sized(blocks: seq<seq<elem>>, bsize: pow2_t)
+    {
+        && (forall i: nat | i < |blocks| :: |blocks[i]| == bsize.full)
+    }
+}
